initial sketch implementation of unification.

src/Ext/ExprCore.v
@@ -1,8 +1,15 @@
 Require Import List Bool.
 Require Import ExtLib.Core.RelDec.
 Require Import ExtLib.Core.Type.
+Require Import ExtLib.Structures.Reducible.
+Require Import ExtLib.Data.List.
+Require Import ExtLib.Data.Option.
+Require Import ExtLib.Data.Monads.OptionMonad.
+Require Import ExtLib.Data.ListNth.
 Require Import ExtLib.Data.HList.
 Require Import ExtLib.Data.Fun.
+Require Import ExtLib.Tactics.Injection.
+Require Import ExtLib.Tactics.EqDep.
 Require Import ExtLib.Tactics.Consider.
 Require Import MirrorCore.EnvI.
 Require Import MirrorCore.ExprI.
@@ -15,13 +22,6 @@ Section env.
 
   Variable types : types.
 
-  Definition typ_cast_val ts (a b : typ) (v : typD types ts a)
-  : option (typD types ts b) :=
-    match typ_cast_typ types (fun x => x) ts a b with
-      | None => None
-      | Some f => Some (f v)
-    end.
-
   Definition func := nat.
   Record tfunction : Type :=
   { tfenv : nat ; tftype : typ }.
@@ -29,12 +29,10 @@ Section env.
   Definition var := nat.
   Definition uvar := nat.
 
-  Unset Elimination Schemes.
-
   Inductive expr : Type :=
   | Var : var -> expr
   | Func : func -> list typ -> expr
-  | App : expr -> list expr -> expr
+  | App : expr -> expr -> expr
   | Abs : typ -> expr -> expr
   | UVar : uvar -> expr
   | Equal : typ -> expr -> expr -> expr
@@ -42,7 +40,7 @@ Section env.
 
   Inductive expr_acc : expr -> expr -> Prop :=
   | acc_App_l : forall f a, expr_acc f (App f a)
-  | acc_App_r : forall f a x, In a x -> expr_acc a (App f x)
+  | acc_App_r : forall f a, expr_acc a (App f a)
   | acc_Abs : forall t e, expr_acc e (Abs t e)
   | acc_Equal_l : forall t l r, expr_acc l (Equal t l r)
   | acc_Equal_r : forall t l r, expr_acc r (Equal t l r)
@@ -50,47 +48,12 @@ Section env.
 
   Definition exprs : Type := list expr.
 
-  Set Elimination Schemes.
-
-  Section expr_ind.
-    Variable P : expr -> Prop.
-    Hypothesis HVar : forall v : var, P (Var v).
-    Hypothesis HFunc : forall f ts, P (Func f ts).
-    Hypothesis HUVar : forall v : var, P (UVar v).
-    Hypothesis HApp : forall f es, P f -> Forall P es -> P (App f es).
-    Hypothesis HAbs : forall t e, P e -> P (Abs t e).
-    Hypothesis HEqual : forall t e1 e2, P e1 -> P e2 -> P (Equal t e1 e2).
-    Hypothesis HNot : forall e, P e -> P (Not e).
-
-    Fixpoint expr_ind x : P x.
-    Proof.
-    refine (
-      match x as x return P x with
-        | Var _ => HVar _
-        | UVar _ => HUVar _
-        | Func _ _ => HFunc _ _
-        | Abs _ _ => HAbs _ (expr_ind _)
-        | App _ _ => HApp (expr_ind _) ((fix all es : Forall P es :=
-          match es with
-            | nil => Forall_nil _
-            | e :: es => Forall_cons _ (expr_ind e) (all es)
-          end) _)
-        | Equal _ _ _ => HEqual _ (expr_ind _) (expr_ind _)
-        | Not _ => HNot (expr_ind _)
-      end).
-    Qed.
-  End expr_ind.
-
   Theorem wf_expr_acc : well_founded expr_acc.
   Proof.
     clear. red.
     induction a; simpl; intros; constructor; intros;
     try solve [ inversion H ].
-    { inversion H0; clear H0; subst; auto.
-      induction es; simpl in *.
-      intuition.
-      destruct H3. subst. inversion H; clear H; subst. auto.
-      eapply IHes; eauto. inversion H; auto. }
+    { inversion H; clear H; subst; auto. }
     { inversion H; clear H; subst; auto. }
     { inversion H; clear H; subst; auto. }
     { inversion H; clear H; subst; auto. }
@@ -108,584 +71,7 @@ Section env.
   Variable funcs : functions.
   Variable meta_env : env (typD types).
 
-  Require Import ExtLib.Data.List.
-  Require Import ExtLib.Data.Option.
-  Require Import ExtLib.Data.Monads.OptionMonad.
-
-  Require Import ExtLib.Structures.Reducible.
-
-  Fixpoint typeof (var_env : tenv typ) (e : expr) {struct e} : option typ :=
-    match e with
-      | Var x =>
-        match nth_error var_env x with
-          | None => None
-          | Some tv => Some tv
-        end
-      | UVar x =>
-        match nth_error meta_env x with
-          | None => None
-          | Some tv => Some (projT1 tv)
-        end
-      | Func f ts =>
-        match nth_error funcs f with
-          | None => None
-          | Some r =>
-(*          if EqNat.beq_nat (length ts) (fenv r) then *)
-              Some (instantiate_typ ts (ftype r))
-(*          else
-              None
-*)
-        end
-      | App e es =>
-        fold_left (fun a n => Monad.bind a (fun a =>
-                              Monad.bind n (fun n =>
-                              type_of_apply a n)))
-                    (map (typeof var_env) es) (typeof var_env e)
-      | Abs t e =>
-        match typeof (t :: var_env) e with
-          | None => None
-          | Some t' => Some (tvArr t t')
-        end
-      | Equal _ _ _ => Some tvProp
-      | Not _ => Some tvProp
-    end.
-
-  (**
-   ** The denotation function with binders must be total because we
-   ** can't introduce the binder until we know that we are going to get
-   ** the right type out, but, at the same time, we don't know we will
-   ** succeed until after we've taken the denotation of the body,
-   ** which we can't do until we have the binder.
-   **
-   **)
-  Fixpoint exprD' (var_env : tenv typ) (e : expr) (t : typ) {struct e} :
-    option (hlist (typD types nil) var_env -> typD types nil t).
-  refine (
-    match e as e return option (hlist (typD types nil) var_env -> typD types nil t) with
-      | Var x =>
-        match nth_error var_env x as z
-          return z = nth_error var_env x ->
-                 option (hlist (typD types nil) var_env -> typD types nil t)
-        with
-          | None => fun _ => None
-          | Some t' => fun pf =>
-            match typ_cast_typ types (fun x => x) _ t' t with
-              | Some f =>
-                Some (fun e => match pf in _ = t''
-                                     return match t'' with
-                                              | Some t => typD types nil t
-                                              | None => unit
-                                            end -> typD types nil t with
-                                 | eq_refl => fun x => f x
-                               end (hlist_nth e x))
-              | None => None
-            end
-        end eq_refl
-      | UVar x =>
-        match lookupAs meta_env x t with
-          | None => None
-          | Some v => Some (fun _ => v)
-        end
-(*
-      | Func f nil =>
-        match nth_error funcs f with
-          | None => None
-          | Some {| fenv := 0 ; ftype := ft ; fdenote := f |} =>
-            Monad.bind (m := option) (typ_cast (fun x => x) _ ft t)
-                       (fun cst => Monad.ret (fun _ => cst f))
-          | Some _ => None
-        end
-*)
-      | Func f ts' =>
-        match nth_error funcs f with
-          | None => None
-          | Some f =>
-            match type_apply _ _ ts' _ _ f.(fdenote) with
-              | None => None
-              | Some t' =>
-                match @typ_cast_val _ (instantiate_typ ts' (ftype f)) t t' with
-                  | Some v => Some (fun _ => v)
-                  | None => None
-                end
-            end
-        end
-      | Abs t' e =>
-        match t as t return option (hlist (typD types nil) var_env -> typD types nil t)
-        with
-          | tvArr lt rt =>
-            match typ_cast_typ types (fun x => x) nil lt t' with
-              | None => None
-              | Some cast =>
-                match @exprD' (lt :: var_env) e rt with
-                  | None => None
-                  | Some a => Some (fun x y => a (Hcons y x))
-                end
-            end
-          | _ => None
-        end
-      | App f xs =>
-        match typeof var_env f with
-          | None => None
-          | Some tf =>
-            match exprD' var_env f tf with
-              | None => None
-              | Some f =>
-                (fix eval_args (t' : typ) (xs : list expr) {struct xs} :
-                  (hlist (typD types nil) var_env -> typD types nil t') ->
-                  option (hlist (typD types nil) var_env -> typD types nil t) :=
-                  match xs with
-                    | nil =>
-                      match typ_cast_typ types (fun x => x) _ t' t with
-                        | None => fun _ => None
-                        | Some cast => fun f => Some (fun g => cast (f g))
-                      end
-                    | x :: xs =>
-                      match t' as t'
-                        return        (hlist (typD types nil) var_env -> typD types nil t') ->
-                               option (hlist (typD types nil) var_env -> typD types nil t)
-                      with
-                        | tvArr tl tr => fun f =>
-                          match exprD' var_env x tl with
-                            | None => None
-                            | Some xv =>
-                              eval_args tr xs (fun e => f e (xv e))
-                          end
-                        | _ => fun _ => None
-                      end
-                  end) tf xs f
-            end
-        end
-      | Equal t' e1 e2 =>
-        match t as t return option (hlist (typD types nil) var_env -> typD types nil t) with
-          | tvProp =>
-            match exprD' var_env e1 t' , exprD' var_env e2 t' with
-              | Some l , Some r =>
-                Some (fun g => (l g) = (r g))
-              (* equal (type := typeFor (typD := typD types) nil t') *)
-              | _ , _ => None
-            end
-          | _ => None
-        end
-      | Not e =>
-        match t as t return option (hlist (typD types nil) var_env -> typD types nil t)
- with
-          | tvProp =>
-            match exprD' var_env e tvProp with
-              | Some P => Some (fun g => not (P g))
-              | _ => None
-            end
-          | _ => None
-        end
-    end).
-  Defined.
-
-
-  Definition exprD (var_env : env (typD types)) (e : expr) (t : typ)
-  : option (typD types nil t) :=
-    let (ts,vs) := split_env var_env in
-    match exprD' ts e t with
-      | None => None
-      | Some f => Some (f vs)
-    end.
-
-  Require Import ExtLib.Tactics.Injection.
-  Require Import ExtLib.Tactics.EqDep.
-  Require Import ExtLib.Data.ListNth.
-
-
-    Theorem split_env_nth_error : forall ve v tv,
-      nth_error ve v = Some tv <->
-      match nth_error (projT1 (split_env ve)) v as t
-      return match t with
-               | Some v => typD types nil v
-               | None => unit
-             end -> Prop
-      with
-        | None => fun _ => False
-        | Some v => fun res => tv = existT _ v res
-      end (hlist_nth (projT2 (split_env ve)) v).
-    Proof.
-      induction ve; simpl; intros.
-      { destruct v; simpl in *; intuition; inversion H. }
-      { destruct v; simpl in *.
-        { intuition.
-          { inversion H; subst. destruct tv; reflexivity. }
-          { subst. destruct a. reflexivity. } }
-        { eapply IHve. } }
-    Qed.
-
-  Theorem exprD_Var : forall ve v t,
-    exprD ve (Var v) t = lookupAs ve v t.
-  Proof.
-    unfold exprD; simpl; intros.
-    consider (split_env ve); intros.
-    unfold lookupAs.
-    generalize (split_env_nth_error ve v).
-    consider (nth_error ve v).
-    { intros. destruct (H1 s); clear H1. clear H3. specialize (H2 eq_refl).
-      rewrite H in *. simpl in *.
-      destruct s; simpl in *.
-      revert H2.
-      change (
-          let f' e0 := hlist_nth e0 v in
-          match
-            nth_error x v as t1
-            return
-            (match t1 with
-               | Some v0 => typD types nil v0
-               | None => unit
-             end -> Prop)
-          with
-            | Some v0 =>
-              fun res : typD types nil v0 =>
-                existT (typD types nil) x0 t0 = existT (typD types nil) v0 res
-            | None => fun _ : unit => False
-          end (f' h) ->
-          match
-            match
-              nth_error x v as z
-              return
-              (z = nth_error x v ->
-               option (hlist (typD types nil) x -> typD types nil t))
-            with
-              | Some t' =>
-                fun pf : Some t' = nth_error x v =>
-                  match typ_cast_typ types (fun x1 : Type => x1) nil t' t with
-                    | Some f =>
-                      Some
-                        (fun e0 : hlist (typD types nil) x =>
-                           match
-                             pf in (_ = t'')
-                             return
-                             (match t'' with
-                                | Some t1 => typD types nil t1
-                                | None => unit
-                              end -> typD types nil t)
-                           with
-                             | eq_refl => fun x1 : typD types nil t' => f x1
-                           end (f' e0))
-                    | None => None
-                  end
-              | None => fun _ : None = nth_error x v => None
-            end eq_refl
-          with
-            | Some f => Some (f h)
-            | None => None
-          end =
-          match typ_cast_typ types (fun x1 : Type => x1) nil x0 t with
-            | Some f => Some (f t0)
-            | None => None
-          end).
-      match goal with
-        | |- context [ @eq_refl ?X ?Y ] =>
-          generalize dependent (@eq_refl X Y)
-      end.
-      pattern (nth_error x v) at 1 5.
-      destruct (nth_error x v).
-      { intro.
-        assert (nth_error x v = Some x0).
-        { cutrewrite (x = projT1 (split_env ve)).
-          rewrite split_env_projT1.
-          erewrite map_nth_error. 2: eassumption. reflexivity.
-          rewrite H. reflexivity. }
-        { assert (x0 = t1).
-          { rewrite H1 in e. inv_all; auto. }
-          subst. destruct (typ_cast_typ types (fun x => x) nil t1 t); auto.
-          { intros. f_equal.
-            subst f'. simpl in *. generalize dependent (hlist_nth h v).
-            generalize dependent (nth_error x v).
-            intros; subst.
-            inv_all. f_equal; auto. } } }
-      { simpl. intro. generalize dependent (hlist_nth h v).
-        rewrite <- e. intuition. } }
-    { intro.
-      assert (nth_error x v = None).
-      { cutrewrite (x = projT1 (split_env ve)).
-        rewrite split_env_projT1.
-        rewrite nth_error_map.
-        rewrite H0. reflexivity.
-        rewrite H. reflexivity. }
-      { match goal with
-          | |- context [ @eq_refl ?X ?Y ] =>
-            generalize dependent (@eq_refl X Y)
-        end.
-        rewrite H; simpl. intros. clear H2.
-        change (
-            let f t' := fun pf : Some t' = nth_error x v =>
-                    match typ_cast_typ types (fun x0 : Type => x0) nil t' t with
-                      | Some f =>
-                        Some
-                          (fun e0 : hlist (typD types nil) x =>
-                             match
-                               pf in (_ = t'')
-                               return
-                               (match t'' with
-                                  | Some t0 => typD types nil t0
-                                  | None => unit
-                                end -> typD types nil t)
-                             with
-                               | eq_refl => fun x0 : typD types nil t' => f x0
-                             end (hlist_nth e0 v))
-                      | None => None
-                    end in
-            match
-              match
-                nth_error x v as z
-                return
-                (z = nth_error x v ->
-                 option (hlist (typD types nil) x -> typD types nil t))
-              with
-                | Some t' => f t'
-                | None => fun _ : None = nth_error x v => None
-              end e
-            with
-              | Some f => Some (f h)
-              | None => None
-            end = None
-          ).
-        intro. clearbody f.
-        revert e.
-        pattern (nth_error x v) at 1 3.
-        rewrite H1. reflexivity. } }
-  Qed.
-
-  Theorem exprD_UVar : forall ve u t,
-    exprD ve (UVar u) t = lookupAs meta_env u t.
-  Proof.
-    unfold exprD. intros.
-    destruct (split_env ve); simpl.
-    destruct (lookupAs meta_env u t); auto.
-  Qed.
-
-  Theorem exprD_Equal : forall ve t l r,
-    exprD ve (Equal t l r) tvProp =
-    match exprD ve l t , exprD ve r t with
-      | Some l , Some r => Some (l = r)
-      | _ , _ => None
-    end.
-  Proof.
-    unfold exprD; intros.
-    destruct (split_env ve); simpl.
-    destruct (exprD' x l t); destruct (exprD' x r t); auto.
-  Qed.
-
-  Theorem exprD_Not : forall ve p,
-    exprD ve (Not p) tvProp =
-    match exprD ve p tvProp with
-      | Some p => Some (~p)
-      | _ => None
-    end.
-  Proof.
-    unfold exprD; intros.
-    destruct (split_env ve); simpl.
-    destruct (exprD' x p tvProp); auto.
-  Qed.
-
-  Fixpoint arrow (ls : list typ) (r : typ) : typ :=
-    match ls with
-      | nil => r
-      | l :: ls => tvArr l (arrow ls r)
-    end.
-
-  Fixpoint apply {ts} {ls : list typ} {r : typ} (f : typD types ts (arrow ls r))
-           (args : hlist (typD types ts) ls) : typD types ts r :=
-    match args in hlist _ ls
-          return typD types ts (arrow ls r) -> typD types ts r
-    with
-      | Hnil => fun x => x
-      | Hcons _ _ v vs => fun x => apply (x v) vs
-    end f.
-
-  Fixpoint mapD {T : Type} {F : T -> Type} (f : forall x, F x) (ls : list T)
-  : hlist F ls :=
-    match ls with
-      | nil => Hnil
-      | l :: ls => @Hcons T F l ls (f l) (mapD f ls)
-    end.
-
-  Fixpoint mapD2 {T U : Type} {F : T -> Type} (f : U -> forall x, F x) (ls : list (U * T))
-  : hlist F (map snd ls) :=
-    match ls as ls return hlist F (map snd ls) with
-      | nil => Hnil
-      | (l,l') :: ls => @Hcons T F _ _ (f l l') (mapD2 f ls)
-    end.
-
-  Theorem exprD_Abs : forall ve t u e val,
-    exprD ve (Abs t e) (tvArr t u) = Some val ->
-    forall x, exprD (existT _ t x :: ve) e u = Some (val x).
-  Proof.
-    unfold exprD. intros.
-    change (split_env (existT (typD types nil) t x :: ve))
-      with (split_env ((existT (typD types nil) t x :: nil) ++ ve)).
-    rewrite split_env_app.
-    destruct (split_env ve). simpl in *.
-    rewrite typ_cast_typ_refl in *.
-    destruct (exprD' (t :: x0) e u); intuition (try congruence).
-    inv_all; subst. reflexivity.
-  Qed.
-
-  Theorem typ_cast_typ_eq : forall f ts t t' v,
-                              typ_cast_typ types f ts t t' = Some v -> t = t'.
-  Proof.
-    clear. unfold typ_cast_typ; simpl; intros.
-    destruct (typ_eq_odec t t'); auto. congruence.
-  Qed.
-
-  Theorem exprD'_typeof : forall e ve t v,
-    exprD' ve e t = Some v ->
-    typeof ve e = Some t.
-  Proof.
-    induction e; simpl; intros; auto;
-    repeat match goal with
-             | [ H : context [ match ?X with _ => _ end ] |- _ ] =>
-               (consider X; intros; try congruence); [ inv_all; subst ]
-           end.
-    { match type of H with
-        | _ ?X = _ => generalize dependent X
-      end.
-      pattern (nth_error ve v) at 1 3.
-      destruct (nth_error ve v); try congruence.
-      intros.
-      match goal with
-        | [ H : context [ match ?X with _ => _ end ] |- _ ] =>
-          (consider X; intros; try congruence); [ inv_all; subst ]
-      end.
-      unfold typ_cast_typ in H.
-      rewrite <- e.
-      destruct (typ_eq_odec t0 t); subst; auto. congruence. }
-    { destruct f0; simpl in *. clear H. f_equal.
-      generalize dependent ftype0.
-      induction ts; simpl; intros.
-      { destruct fenv0; simpl in *. inv_all; subst.
-        Lemma typ_cast_val_eq : forall ts a b v v', 
-                                  typ_cast_val ts a b v = Some v' ->
-                                  a = b.
-        Proof.
-          clear. unfold typ_cast_val; simpl; intros.
-          unfold typ_cast_typ in *. generalize (@typ_eq_odec_None a b).
-          destruct (typ_eq_odec a b); auto. congruence.
-        Qed.
-        eapply typ_cast_val_eq in H1. auto. congruence. }
-      { destruct fenv0; simpl in *; try congruence.
-        match goal with
-          | H : match ?X with _ => _ end = _ |- _ =>
-            consider X
-        end; intros; try congruence.
-        inv_all; subst.
-        specialize (IHts _ fdenote0). unfold typ_cast_val in *.
-        unfold typ_cast_typ in *.
-        generalize (@typ_eq_odec_None (subst0_typ a (instantiate_typ ts ftype0)) t).
-        destruct (typ_eq_odec (subst0_typ a (instantiate_typ ts ftype0)) t); try congruence. } }
-    { unfold lookupAs in *.
-      destruct (nth_error meta_env v).
-      { destruct s. simpl in *.
-        unfold typ_cast_typ in *.
-        destruct (typ_eq_odec x t); subst; auto.
-        congruence. }
-      { congruence. } }
-    { clear H1 H0 IHe. generalize dependent t0. generalize dependent t. clear - H.
-      induction H; simpl; intros.
-      { generalize (@typ_cast_typ_eq (fun x => x) nil t0 t).
-        destruct (typ_cast_typ types (fun x : Type => x) nil t0 t); try congruence.
-        inv_all. subst. intros. specialize (H _ eq_refl). subst; auto. }
-      { destruct t0; try congruence.
-        consider (exprD' ve x t0_1); try congruence; intros. eapply H in H1.
-        rewrite H1 in *. simpl in *.
-        change (typ_eqb t0_1 t0_1) with (t0_1 ?[ eq ] t0_1).
-        consider (t0_1 ?[ eq ] t0_1); try congruence; intros.
-        clear H3. eapply IHForall; eauto. } }
-    { eapply IHe in H0.
-      generalize (typ_cast_typ_eq (fun x => x) nil t1 t H); intros; subst.
-      rewrite H0. reflexivity. }
-    { destruct t0; auto; congruence. }
-    { destruct t; auto; congruence. }
-  Qed.
-
-  Theorem exprD_app_nil : forall ve t e,
-    exprD ve (App e nil) t = exprD ve e t.
-  Proof.
-    unfold exprD; simpl; intros.
-    destruct (split_env ve); simpl in *.
-    consider (exprD' x e t); intros.
-    { rewrite (exprD'_typeof _ _ H).
-      rewrite H.
-      rewrite typ_cast_typ_refl. reflexivity. }
-    { consider (typeof x e); intros; auto.
-      { unfold typ_cast_typ.
-        destruct (typ_eq_odec t0 t); subst.
-        { rewrite H. reflexivity. }
-        { destruct (exprD' x e t0); auto. } } }
-  Qed.
-
-  Theorem exprD_App : forall ve t e args,
-    exprD ve (App e args) t =
-    match typeof (map (@projT1 _ _) ve) e with
-      | None => None
-      | Some tf =>
-        match exprD ve e tf with
-          | None => None
-          | Some f =>
-            (fix eval_args (tf : typ) (f : typD types nil tf) (args : list expr)
-                 {struct args}
-             : option (typD types nil t) :=
-               match args with
-                 | nil => typ_cast_val nil tf t f
-                 | arg :: args =>
-                   match tf as tf
-                         return typD types nil tf -> option (typD types nil t)
-                   with
-                     | tvArr l r => fun f =>
-                       match exprD ve arg l with
-                         | None => None
-                         | Some argv =>
-                           eval_args r (f argv) args
-                       end
-                     | _ => fun _ => None
-                   end f
-               end) tf f args
-        end
-    end.
-  Proof.
-    intros; simpl.
-    unfold exprD; simpl; intros.
-    rewrite <- split_env_projT1.
-    destruct (split_env ve); simpl in *; intros.
-    destruct (typeof x e); auto.
-    destruct (exprD' x e t0); auto.
-    clear. generalize dependent t0.
-    induction args; simpl; intros.
-    { unfold typ_cast_val.
-      destruct (typ_cast_typ types (fun x0 : Type => x0) nil t0 t); auto. }
-    { destruct t0; auto.
-      destruct (exprD' x a t0_1); auto.
-      rewrite IHargs. reflexivity. }
-  Qed.
-
-  Fixpoint anyb {T} (p : T -> bool) (ls : list T) : bool :=
-    match ls with
-      | nil => false
-      | l :: ls => if p l then true else anyb p ls
-    end.
-
-  Fixpoint mentionsU (u : nat) (e : expr) {struct e} : bool :=
-    match e with
-      | Var _
-      | Func _ _ => false
-      | UVar u' => EqNat.beq_nat u u'
-      | App f es =>
-        if mentionsU u f then true else
-          (fix anyb ls : bool :=
-            match ls with
-              | nil => false
-              | l :: ls => if mentionsU u l then true else anyb ls
-            end) es
-      | Abs _ e => mentionsU u e
-      | Equal _ e1 e2 => if mentionsU u e1 then true else mentionsU u e2
-      | Not e => mentionsU u e
-    end.
-
-  Fixpoint expr_eq_dec (e1 e2 : expr) : bool.
-  refine (
+  Fixpoint expr_eq_dec (e1 e2 : expr) : bool :=
     match e1 , e2 with
       | Var v1 , Var v2 => EqNat.beq_nat v1 v2
       | UVar v1 , UVar v2 => EqNat.beq_nat v1 v2
@@ -693,15 +79,9 @@ Section env.
         if EqNat.beq_nat f1 f2 then
           ts1 ?[ eq ] ts2
         else false
-      | App f1 es1 , App f2 es2 =>
+      | App f1 e1 , App f2 e2 =>
         if expr_eq_dec f1 f2 then
-          (fix check es1 es2 : bool :=
-            match es1 , es2 with
-              | nil , nil => true
-              | e1 :: es1 , e2 :: es2 =>
-                if expr_eq_dec e1 e2 then check es1 es2 else false
-              | _ , _ => false
-            end) es1 es2
+          expr_eq_dec e1 e2
         else
           false
       | Abs t1 e1 , Abs t2 e2 =>
@@ -716,48 +96,27 @@ Section env.
         else false
       | Not e1 , Not e2 => expr_eq_dec e1 e2
       | _ , _ => false
-    end).
-  Defined.
+    end.
 
   Theorem expr_eq_dec_eq : forall e1 e2,
     expr_eq_dec e1 e2 = true <-> e1 = e2.
   Proof.
-    induction e1; destruct e2; simpl; intros; try solve [ intuition congruence ].
-    { consider (EqNat.beq_nat v v0); intros; subst; intuition. inversion H0; subst; auto. }
-    { consider (EqNat.beq_nat f f0); intros; subst.
-      { change (ts ?[ eq ] l = true <-> Func f0 ts = Func f0 l).
-        consider (ts ?[ eq ] l). intros; subst. intuition.
-        intuition congruence. }
-      { intuition congruence. } }
-    { consider (EqNat.beq_nat v u); subst; intuition congruence. }
-    { consider (expr_eq_dec e1 e2); intros.
-      { eapply IHe1 in H0. subst.
-        generalize dependent l. clear - H.
-        induction H; simpl; intros.
-        { destruct l; intuition congruence. }
-        { destruct l0; try intuition congruence.
-          consider (expr_eq_dec x e).
-          rewrite IHForall. intros. eapply H in H1. subst; f_equal.
-          intuition; inversion H1; subst; auto.
-          intros. intuition.
-          inversion H2; subst.
-          rewrite <- H1. eapply H. reflexivity. } }
-      { intuition. inversion H1; subst. rewrite <- H0. apply IHe1. reflexivity. } }
-    { change typ_eqb with (@rel_dec _ _ _) in *. consider (t ?[ eq ] t0).
-      intros; subst. intuition try congruence.
-      eapply IHe1 in H; congruence.
-      inversion H; subst.
-      eapply IHe1. reflexivity.
-      intros. intuition congruence. }
-    { change typ_eqb with (@rel_dec _ _ _) in *.
-      specialize (IHe1_1 e2_1). specialize (IHe1_2 e2_2).
-      consider (t ?[ eq ] t0);
-      consider (expr_eq_dec e1_1 e2_1);
-      consider (expr_eq_dec e1_2 e2_2); intros; subst; intuition try congruence; subst.
-      inversion H5; subst; auto.
-      inversion H4; subst; auto.
-      inversion H2; subst; auto. }
-    { rewrite IHe1. intuition congruence. }
+    induction e1; destruct e2; simpl; intros;
+    repeat match goal with
+             | |- context [ if ?X then ?Y else false ] =>
+               change (if X then Y else false) with (andb X Y)
+             | |- context [ EqNat.beq_nat ?X ?Y ] =>
+               change (EqNat.beq_nat X Y) with (X ?[ eq ] Y) ;
+                 rewrite rel_dec_correct
+             | |- context [ typ_eqb ?X ?Y ] =>
+               change (typ_eqb X Y) with (X ?[ eq ] Y) ;
+                 rewrite rel_dec_correct
+             | |- context [ RelDec.list_eq RelDec_eq_typ ?X ?Y ] =>
+               change (RelDec.list_eq RelDec_eq_typ X Y) with (X ?[ eq ] Y) ;
+                 rewrite rel_dec_correct
+             | |- _ => rewrite andb_true_iff
+             | H : forall x, (_ = true) <-> _ |- _ => rewrite H
+           end; try solve [ intuition congruence ].
   Qed.
 
   Global Instance RelDec_eq_expr : RelDec (@eq expr) :=
@@ -770,6 +129,7 @@ Section env.
 
 End env.
 
+(*
 Section expr.
   Variable types : types.
 
@@ -779,3 +139,4 @@ Section expr.
   ; wf_acc := wf_expr_acc
   }.
 End expr.
+*)
