src/Ext/ExprD3.v
@@ -1,0 +1,652 @@
+Require Import ExtLib.Core.RelDec.
+Require Import ExtLib.Data.HList.
+Require Import ExtLib.Data.ListNth.
+Require Import ExtLib.Data.Monads.OptionMonad.
+Require Import ExtLib.Tactics.Consider.
+Require Import ExtLib.Tactics.Injection.
+Require Import ExtLib.Tactics.EqDep.
+Require Import MirrorCore.EnvI.
+Require Import MirrorCore.ExprI.
+Require Import MirrorCore.Ext.Types.
+Require Import MirrorCore.Ext.ExprCore.
+Require Import MirrorCore.Ext.ExprDI.
+Require Import MirrorCore.Ext.ExprT.
+
+Set Implicit Arguments.
+Set Strict Implicit.
+
+Module EXPR_DENOTE_3 <: ExprDenote.
+
+  Create HintDb exprD_rw discriminated.
+
+  Section with_envs.
+    Variable ts : types.
+    Variable fs : functions ts.
+    Variable us : env (typD ts).
+
+  Fixpoint exprD_simul' (var_env : tenv typ) (e : expr) {struct e} :
+    option { t : typ & hlist (typD ts nil) var_env -> typD ts nil t } :=
+    let Z t := hlist (typD ts nil) var_env -> typD ts nil t in
+    match e return option { t : typ & hlist (typD ts nil) var_env -> typD ts nil t } with
+      | Var x =>
+        match nth_error var_env x as pf
+          return pf = nth_error var_env x ->
+                 option { t : typ & hlist (typD ts nil) var_env -> typD ts nil t }
+        with
+          | None => fun _ => None
+          | Some t => fun pf =>
+            Some (existT _ t (fun e => match pf in _ = t''
+                                           return match t'' with
+                                                    | Some t => typD ts nil t
+                                                    | None => unit
+                                                  end -> typD ts nil t with
+                                       | eq_refl => fun x => x
+                                     end (hlist_nth e x)))
+        end eq_refl
+      | UVar x =>
+        match nth_error us x with
+          | None => None
+          | Some (existT t v) => Some (existT Z t (fun _ => v))
+        end
+      | Func f ts' =>
+        match nth_error fs f with
+          | None => None
+          | Some f =>
+            match type_apply _ _ ts' _ _ f.(fdenote) with
+              | None => None
+              | Some v =>
+                Some (existT Z (instantiate_typ ts' (ftype f)) (fun _ => v))
+            end
+        end
+      | Abs t' e =>
+        match exprD_simul' (t' :: var_env) e with
+          | None => None
+          | Some (existT t v) =>
+            Some (existT (fun t => hlist (typD ts nil) var_env -> typD ts nil t) (tvArr t' t) (fun g x => v (Hcons x g)))
+        end
+      | App f x =>
+        match exprD_simul' var_env f with
+          | None => None
+          | Some (existT (tvArr l r) f) =>
+            match exprD' var_env x l with
+              | None => None
+              | Some x => Some (existT (fun t => hlist (typD ts nil) var_env -> typD ts nil t) r (fun v => (f v) (x v)))
+            end
+          | _ => None
+        end
+      | Equal t e1 e2 =>
+        match exprD' var_env e1 t , exprD' var_env e2 t with
+          | Some v1, Some v2 =>
+            Some (existT Z tvProp (fun v => @eq _ (v1 v) (v2 v)))
+          | _ , _ => None
+        end
+      | Not e =>
+        match exprD' var_env e tvProp with
+          | None => None
+          | Some P => Some (existT Z tvProp (fun v => not (P v)))
+        end
+    end
+  with exprD' (var_env : tenv typ) (e : expr) (t : typ) {struct e} :
+    option (hlist (typD ts nil) var_env -> typD ts nil t) :=
+    match e with
+      | Var x =>
+        match nth_error var_env x as z
+          return z = nth_error var_env x ->
+                 option (hlist (typD ts nil) var_env -> typD ts nil t)
+        with
+          | None => fun _ => None
+          | Some t' => fun pf =>
+            match typ_cast_typ ts (fun x => x) _ t' t with
+              | Some f =>
+                Some (fun e => match pf in _ = t''
+                                     return match t'' with
+                                              | Some t => typD ts nil t
+                                              | None => unit
+                                            end -> typD ts nil t with
+                                 | eq_refl => fun x => f x
+                               end (hlist_nth e x))
+              | None => None
+            end
+        end eq_refl
+      | UVar x =>
+        match lookupAs us x t with
+          | None => None
+          | Some v => Some (fun _ => v)
+        end
+      | Func f ts' =>
+        match nth_error fs f with
+          | None => None
+          | Some f =>
+            match type_apply _ _ ts' _ _ f.(fdenote) with
+              | None => None
+              | Some t' =>
+                match @typ_cast_val _ _ (instantiate_typ ts' (ftype f)) t t' with
+                  | Some v => Some (fun _ => v)
+                  | None => None
+                end
+            end
+        end
+      | Abs t' e =>
+        match t as t return option (hlist (typD ts nil) var_env -> typD ts nil t)
+        with
+          | tvArr lt rt =>
+            match typ_cast_typ ts (fun x => x) nil lt t' with
+              | None => None
+              | Some cast =>
+                match @exprD' (lt :: var_env) e rt with
+                  | None => None
+                  | Some a => Some (fun x y => a (Hcons y x))
+                end
+            end
+          | _ => None
+        end
+      | App f x =>
+        match exprD_simul' var_env f with
+          | Some (existT (tvArr l r) f) =>
+            match exprD' var_env x l with
+              | None => None
+              | Some x =>
+                match typ_cast_typ ts (fun x => x) _ r t with
+                  | None => None
+                  | Some cast => Some (fun v => cast ((f v) (x v)))
+                end
+            end
+          | _ => None
+        end
+      | Not e =>
+        match t as t
+              return option (hlist (typD ts nil) var_env -> typD ts nil t)
+        with
+          | tvProp => match exprD' var_env e tvProp with
+                        | None => None
+                        | Some P => Some (fun v => not (P v))
+                      end
+          | _ => None
+        end
+      | Equal t' e1 e2 =>
+        match t as t return option (hlist (typD ts nil) var_env -> typD ts nil t) with
+          | tvProp =>
+            match exprD' var_env e1 t' , exprD' var_env e2 t' with
+              | Some l , Some r =>
+                Some (fun g => (l g) = (r g))
+              (* equal (type := typeFor (typD := typD ts) nil t') *)
+              | _ , _ => None
+            end
+          | _ => None
+        end
+    end.
+
+  Definition exprD (var_env : env (typD ts)) (e : expr) (t : typ)
+  : option (typD ts nil t) :=
+    let (ts,vs) := split_env var_env in
+    match exprD' ts e t with
+      | None => None
+      | Some f => Some (f vs)
+    end.
+
+    Theorem split_env_nth_error : forall ve v tv,
+      nth_error ve v = Some tv <->
+      match nth_error (projT1 (split_env ve)) v as t
+      return match t with
+               | Some v => typD ts nil v
+               | None => unit
+             end -> Prop
+      with
+        | None => fun _ => False
+        | Some v => fun res => tv = existT _ v res
+      end (hlist_nth (projT2 (split_env ve)) v).
+    Proof.
+      induction ve; simpl; intros.
+      { destruct v; simpl in *; intuition; inversion H. }
+      { destruct v; simpl in *.
+        { intuition.
+          { inversion H; subst. destruct tv; reflexivity. }
+          { subst. destruct a. reflexivity. } }
+        { eapply IHve. } }
+    Qed.
+
+  Theorem exprD_Var : forall ve v t,
+    exprD ve (Var v) t = lookupAs ve v t.
+  Proof.
+    unfold exprD; simpl; intros.
+    consider (split_env ve); intros.
+    unfold lookupAs.
+    generalize (split_env_nth_error ve v).
+    consider (nth_error ve v).
+    { intros. destruct (H1 s); clear H1. clear H3. specialize (H2 eq_refl).
+      rewrite H in *. simpl in *.
+      destruct s; simpl in *.
+      revert H2.
+      change (
+          let f' e0 := hlist_nth e0 v in
+          match
+            nth_error x v as t1
+            return
+            (match t1 with
+               | Some v0 => typD ts nil v0
+               | None => unit
+             end -> Prop)
+          with
+            | Some v0 =>
+              fun res : typD ts nil v0 =>
+                existT (typD ts nil) x0 t0 = existT (typD ts nil) v0 res
+            | None => fun _ : unit => False
+          end (f' h) ->
+          match
+            match
+              nth_error x v as z
+              return
+              (z = nth_error x v ->
+               option (hlist (typD ts nil) x -> typD ts nil t))
+            with
+              | Some t' =>
+                fun pf : Some t' = nth_error x v =>
+                  match typ_cast_typ ts (fun x1 : Type => x1) nil t' t with
+                    | Some f =>
+                      Some
+                        (fun e0 : hlist (typD ts nil) x =>
+                           match
+                             pf in (_ = t'')
+                             return
+                             (match t'' with
+                                | Some t1 => typD ts nil t1
+                                | None => unit
+                              end -> typD ts nil t)
+                           with
+                             | eq_refl => fun x1 : typD ts nil t' => f x1
+                           end (f' e0))
+                    | None => None
+                  end
+              | None => fun _ : None = nth_error x v => None
+            end eq_refl
+          with
+            | Some f => Some (f h)
+            | None => None
+          end =
+          match typ_cast_typ ts (fun x1 : Type => x1) nil x0 t with
+            | Some f => Some (f t0)
+            | None => None
+          end).
+      match goal with
+        | |- context [ @eq_refl ?X ?Y ] =>
+          generalize dependent (@eq_refl X Y)
+      end.
+      pattern (nth_error x v) at 1 5.
+      destruct (nth_error x v).
+      { intro.
+        assert (nth_error x v = Some x0).
+        { cutrewrite (x = projT1 (split_env ve)).
+          rewrite split_env_projT1.
+          erewrite map_nth_error. 2: eassumption. reflexivity.
+          rewrite H. reflexivity. }
+        { assert (x0 = t1).
+          { rewrite H1 in e. inv_all; auto. }
+          subst. destruct (typ_cast_typ ts (fun x => x) nil t1 t); auto.
+          { intros. f_equal.
+            subst f'. simpl in *. generalize dependent (hlist_nth h v).
+            generalize dependent (nth_error x v).
+            intros; subst.
+            inv_all. f_equal; auto. } } }
+      { simpl. intro. generalize dependent (hlist_nth h v).
+        rewrite <- e. intuition. } }
+    { intro.
+      assert (nth_error x v = None).
+      { cutrewrite (x = projT1 (split_env ve)).
+        rewrite split_env_projT1.
+        rewrite nth_error_map.
+        rewrite H0. reflexivity.
+        rewrite H. reflexivity. }
+      { match goal with
+          | |- context [ @eq_refl ?X ?Y ] =>
+            generalize dependent (@eq_refl X Y)
+        end.
+        rewrite H; simpl. intros. clear H2.
+        change (
+            let f t' := fun pf : Some t' = nth_error x v =>
+                    match typ_cast_typ ts (fun x0 : Type => x0) nil t' t with
+                      | Some f =>
+                        Some
+                          (fun e0 : hlist (typD ts nil) x =>
+                             match
+                               pf in (_ = t'')
+                               return
+                               (match t'' with
+                                  | Some t0 => typD ts nil t0
+                                  | None => unit
+                                end -> typD ts nil t)
+                             with
+                               | eq_refl => fun x0 : typD ts nil t' => f x0
+                             end (hlist_nth e0 v))
+                      | None => None
+                    end in
+            match
+              match
+                nth_error x v as z
+                return
+                (z = nth_error x v ->
+                 option (hlist (typD ts nil) x -> typD ts nil t))
+              with
+                | Some t' => f t'
+                | None => fun _ : None = nth_error x v => None
+              end e
+            with
+              | Some f => Some (f h)
+              | None => None
+            end = None
+          ).
+        intro. clearbody f.
+        revert e.
+        pattern (nth_error x v) at 1 3.
+        rewrite H1. reflexivity. } }
+  Qed.
+
+  Theorem exprD_UVar : forall ve u t,
+    exprD ve (UVar u) t = lookupAs us u t.
+  Proof.
+    unfold exprD. intros.
+    destruct (split_env ve); simpl.
+    destruct (lookupAs us u t); auto.
+  Qed.
+
+  Theorem exprD_Func : forall ve f ts t,
+    exprD ve (Func f ts) t =
+    match nth_error fs f with
+      | None => None
+      | Some f =>
+        match type_apply _ _ ts _ _ f.(fdenote) with
+          | None => None
+          | Some t' =>
+            @typ_cast_val _ _ (instantiate_typ ts (ftype f)) t t'
+        end
+    end.
+  Proof.
+    unfold exprD; intros.
+    destruct (split_env ve); simpl.
+    destruct (nth_error fs f); auto.
+    destruct (type_apply ts (fenv f0) ts0 nil (ftype f0) (fdenote f0)); auto.
+    destruct (typ_cast_val ts nil (instantiate_typ ts0 (ftype f0)) t t0); auto.
+  Qed.
+
+  Theorem exprD_Equal : forall ve t l r t',
+    exprD ve (Equal t l r) t' =
+    match t' as t' return option (typD ts nil t') with
+      | tvProp =>
+        match exprD ve l t , exprD ve r t with
+          | Some l , Some r => Some (l = r)
+          | _ , _ => None
+        end
+      | _ => None
+    end.
+  Proof.
+    unfold exprD; intros.
+    destruct (split_env ve); simpl.
+    destruct t'; auto.
+    destruct (exprD' x l t); destruct (exprD' x r t); auto.
+  Qed.
+
+  Theorem exprD_Not : forall ve p t',
+    exprD ve (Not p) t' =
+    match t' as t' return option (typD ts nil t') with
+      | tvProp =>
+        match exprD ve p tvProp with
+          | Some p => Some (~p)
+          | _ => None
+        end
+      | _ => None
+    end.
+  Proof.
+    unfold exprD; intros.
+    destruct (split_env ve); simpl.
+    destruct t'; auto.
+    destruct (exprD' x p tvProp); auto.
+  Qed.
+
+(*
+   Theorem exprD_Abs_eq : forall ve t t' e val,
+      exprD ve (Abs t e) t' = Some val <->
+      match t' as t' return typD ts nil t' -> Prop with
+        | tvArr l r => fun val =>
+           match typ_cast_typ ts (fun x => x) nil l t with
+             | None => False
+             | Some cast =>
+               forall x, exprD (existT _ t (cast x) :: ve) e r = Some (val x)
+           end
+        | _ => fun _ => False
+      end val.
+   Proof.
+    unfold exprD. intros.
+    destruct t'; simpl; try (destruct (split_env ve); intuition congruence).
+    match goal with
+      | |- (let (_,_) := _ in
+            match match ?X with _ => _ end with _ => _ end) = _
+           <->
+           match ?Y with _ => _ end =>
+        change X with Y; consider Y; intros
+    end.
+    { generalize (typ_cast_typ_eq _ _ _ _ _ H).
+      destruct (split_env ve). intros. subst. simpl.
+      destruct (exprD' (t :: x) e t'2).
+      { admit. }
+      { intuition try congruence.
+ }
+    { destruct (split_env ve). intuition congruence. }
+  Qed.
+*)
+
+  (** TODO: This definition is too weak **)
+   Theorem exprD_Abs : forall ve t u e val,
+      exprD ve (Abs t e) (tvArr t u) = Some val ->
+      forall x, exprD (existT _ t x :: ve) e u = Some (val x).
+   Proof.
+    unfold exprD. intros.
+    change (split_env (existT (typD ts nil) t x :: ve))
+      with (split_env ((existT (typD ts nil) t x :: nil) ++ ve)).
+    rewrite split_env_app.
+    destruct (split_env ve). simpl in *.
+    rewrite typ_cast_typ_refl in *.
+    destruct (exprD' (t :: x0) e u); intuition (try congruence).
+    inv_all; subst. reflexivity.
+  Qed.
+
+   Lemma exprD'_exprD_simul' : forall e ve t val,
+     exprD_simul' ve e = Some (@existT _ _ t val) ->
+     exprD' ve e t = Some val.
+   Proof.
+     induction e; simpl; intros.
+     { match goal with
+         | H : context [ @eq_refl ?X ?Y ] |- _ =>
+           generalize dependent (@eq_refl X Y)
+       end.
+       pattern (nth_error ve v) at 1 3 7.
+       destruct (nth_error ve v); try congruence.
+       intros. inv_all. destruct H. subst. subst.
+       rewrite typ_cast_typ_refl. reflexivity. }
+     { destruct (nth_error fs f); try intuition congruence.
+       destruct (type_apply ts (fenv f0) l nil (ftype f0) (fdenote f0));
+         try congruence.
+       inv_all. destruct H; subst. subst.
+       unfold typ_cast_val. rewrite typ_cast_typ_refl. reflexivity. }
+     { specialize (IHe1 ve).
+       destruct (exprD_simul' ve e1); try intuition congruence.
+       destruct s. specialize (IHe1 x t0 eq_refl).
+       destruct x; try congruence.
+       destruct (exprD' ve e2 x1); try congruence.
+       inv_all. destruct H; subst. subst.
+       rewrite typ_cast_typ_refl. reflexivity. }
+     { specialize (IHe (t :: ve)).
+       destruct (exprD_simul' (t :: ve) e); try congruence. destruct s.
+       inv_all. destruct H; subst. subst.
+       rewrite typ_cast_typ_refl.
+       rewrite (IHe _ _ eq_refl). reflexivity. }
+     { unfold lookupAs. destruct (nth_error us u); try congruence.
+       destruct s. inv_all. destruct H. subst. subst.
+       simpl. rewrite typ_cast_typ_refl. reflexivity. }
+     { specialize (IHe1 ve). specialize (IHe2 ve).
+       destruct (exprD' ve e1 t); try congruence.
+       destruct (exprD' ve e2 t); try congruence.
+       inv_all. destruct H. subst. subst. reflexivity. }
+     { specialize (IHe ve). destruct (exprD' ve e tvProp); try congruence.
+       inv_all. destruct H; subst. f_equal. auto. }
+   Qed.
+
+  Hint Rewrite exprD_Var exprD_UVar exprD_Equal exprD_Not exprD_Func : exprD_rw.
+
+   Lemma exprD'_typeof : forall e ve t val,
+     exprD' ve e t = Some val ->
+     typeof_expr (typeof_funcs fs) (typeof_env us) ve e = Some t.
+   Proof.
+     induction e; simpl; intros.
+     { admit. }
+     { destruct (nth_error fs f); try congruence.
+       admit. }
+     { specialize (IHe1 ve).
+       consider (exprD_simul' ve e1); try congruence; intros.
+       destruct s. destruct x; try congruence.
+       eapply exprD'_exprD_simul' in H.
+       eapply IHe1 in H. rewrite H.
+       specialize (IHe2 ve x1).
+       destruct (exprD' ve e2 x1); try congruence.
+       specialize (IHe2 _ eq_refl). rewrite IHe2.
+       simpl. change (typ_eqb x1 x1) with (x1 ?[ eq ] x1).
+       rewrite rel_dec_eq_true; eauto with typeclass_instances.
+       match goal with
+         | H : match ?X with _ => _ end = _ |- _ =>
+           consider X; intros; try congruence
+       end.
+       generalize (@typ_cast_typ_eq _ _ _ _ _ _ H0). congruence. }
+     { destruct t0; try congruence.
+       specialize (IHe (t :: ve) t0_2).
+       match goal with
+         | H : match ?X with _ => _ end = _ |- _ =>
+           consider X; intros; try congruence
+       end.
+       generalize (@typ_cast_typ_eq _ _ _ _ _ _ H); intro; subst.
+       destruct (exprD' (t :: ve) e t0_2); try congruence.
+       erewrite IHe; eauto. }
+     { unfold lookupAs, typeof_env in *.
+       rewrite nth_error_map.
+       destruct (nth_error us u); try congruence.
+       destruct s; simpl.
+       repeat match goal with
+                | H : match ?X with _ => _ end = _ |- _ =>
+                  consider X; intros; try congruence
+              end.
+       specialize (typ_cast_typ_eq _ _ _ _  _ H). congruence. }
+     { destruct t0; try congruence.
+       specialize (IHe1 ve t). specialize (IHe2 ve t).
+       destruct (exprD' ve e1 t); try congruence.
+       destruct (exprD' ve e2 t); try congruence.
+       erewrite IHe1 by eauto.
+       erewrite IHe2 by eauto.
+       change typ_eqb with (@rel_dec _ (@eq typ) _).
+       rewrite rel_dec_eq_true by eauto with typeclass_instances.
+       reflexivity. }
+     { destruct t; try congruence.
+       specialize (IHe ve tvProp).
+       destruct (exprD' ve e tvProp); try congruence.
+       erewrite IHe by eauto. reflexivity. }
+   Qed.
+
+   Lemma exprD'_typeof_None : forall e ve t,
+     exprD' ve e t = None ->
+     typeof_expr (typeof_funcs fs) (typeof_env us) ve e <> Some t.
+   Proof.
+     induction e; simpl; intros.
+     { admit. }
+     { unfold typeof_funcs. rewrite nth_error_map.
+       destruct (nth_error fs f); try congruence.
+       destruct f0; simpl in *.
+       match goal with
+         | H : match ?X with _ => _ end = _ |- _ =>
+           consider X; intros
+       end.
+       rewrite (type_apply_length_equal' _ _ _ _ _ _ H).
+       consider (EqNat.beq_nat fenv fenv); try congruence.
+       match goal with
+         | H : match ?X with _ => _ end = _ |- _ =>
+           consider X; try congruence; intros
+       end.
+       intro. inv_all. subst. eapply typ_cast_val_refl; eauto.
+       consider (EqNat.beq_nat (length l) fenv); try congruence; intros.
+       destruct (@type_apply_length_equal ts ftype l fenv nil fdenote H1).
+       clear - H H2.
+       match type of H with 
+         | ?T = _ =>
+           match type of H2 with
+             | ?T' = _ =>
+               change T with T in *
+           end
+       end.
+       rewrite H in H2. congruence. }
+     { consider (exprD_simul' ve e1); intros.
+       destruct s. eapply exprD'_exprD_simul' in H.
+       admit. admit. }
+   Admitted.
+
+  Theorem typeof_exprD : forall vs e t,
+    typeof_expr (typeof_funcs fs) (typeof_env us) (typeof_env vs) e = Some t ->
+    exists val, exprD vs e t = Some val.
+  Proof.
+    intros vs e; revert vs.
+    induction e; simpl; intros; autorewrite with exprD_rw;
+      unfold lookupAs, typeof_funcs, typeof_env in *;
+      repeat match goal with
+               | H : _ |- _ => rewrite nth_error_map in H
+               | _ : match ?X with _ => _ end = _ |- _ =>
+                 (consider X; try congruence); [ intros ]
+               | |- _ => progress (inv_all; subst; simpl in *)
+               | H : sigT _ |- _ => destruct H
+               | |- _ => rewrite typ_cast_typ_refl
+               | H : forall x, _ = _ -> _ |- _ =>
+                 specialize (H _ eq_refl)
+               | H : forall x y, _ = _ -> _ |- _ =>
+                 specialize (H _ _ eq_refl)
+               | H : exists x, _ |- _ =>
+                 destruct H
+               | H : _ |- _ =>
+                 erewrite H by eauto
+             end; eauto.
+  Admitted.
+
+   Theorem exprD_App : forall ve t e arg,
+      exprD ve (App e arg) t =
+      match typeof_expr (typeof_funcs fs) (typeof_env us) (typeof_env ve) e with
+        | Some (tvArr l r) =>
+          match exprD ve e (tvArr l r) , exprD ve arg l , typ_cast_typ ts (fun x => x) nil r t with
+            | Some f , Some x , Some cast =>
+              Some (cast (f x))
+            | _ , _ , _ => None
+          end
+        | _ => None
+      end.
+   Proof.
+     unfold exprD; intros.
+     unfold typeof_env in *.
+     rewrite <- (split_env_projT1 ve).
+     destruct (split_env ve); simpl.
+     consider (exprD_simul' x e); intros.
+     { destruct s.
+       generalize (exprD'_exprD_simul' _ H); intro.
+       generalize (exprD'_typeof _ _ H0).
+       unfold typeof_env; intro; rewrite H1.
+       destruct x0; auto. rewrite H0.
+       destruct (exprD' x arg x0_1); auto.
+       clear.
+       destruct (typ_cast_typ ts (fun x0 : Type => x0) nil x0_2 t); auto. }
+     { admit. }
+   Qed.
+
+  End with_envs.
+End EXPR_DENOTE_3.
+
+Import EXPR_DENOTE_3.
+Export EXPR_DENOTE_3.
+
+Instance Expr_expr ts (fs : functions ts) : Expr (typD ts) expr :=
+{ exprD := exprD fs
+; acc := expr_acc
+; wf_acc := wf_expr_acc
+}.
+
+Create HintDb exprD_rw discriminated.
+Hint Rewrite exprD_Var exprD_App exprD_UVar exprD_Equal exprD_Not exprD_Func : exprD_rw.
