src/Ext/ExprDI.v
@@ -1,0 +1,94 @@
+Require Import ExtLib.Core.RelDec.
+Require Import MirrorCore.EnvI.
+Require Import MirrorCore.ExprI.
+Require Import MirrorCore.Ext.Types.
+Require Import MirrorCore.Ext.ExprCore.
+Require Import MirrorCore.Ext.ExprT.
+
+Set Implicit Arguments.
+Set Strict Implicit.
+
+Module Type ExprDenote.
+
+  (**
+   ** The denotation function with binders must be total because we
+   ** can't introduce the binder until we know that we are going to get
+   ** the right type out, but, at the same time, we don't know we will
+   ** succeed until after we've taken the denotation of the body,
+   ** which we can't do until we have the binder.
+   **
+   **)
+  Parameter exprD : forall (ts : types) (fs : functions ts),
+    env (typD ts) -> env (typD ts) -> expr -> forall t : typ,
+    option (typD ts nil t).
+
+  Section with_envs.
+    Variable ts : types.
+    Variable fs : functions ts.
+    Variable us : env (typD ts).
+
+    Axiom typeof_exprD : forall vs e t,
+      typeof_expr (typeof_funcs fs) (typeof_env us) (typeof_env vs) e = Some t ->
+      exists val, exprD fs us vs e t = Some val.
+
+    Axiom exprD_Var : forall ve v t,
+      exprD fs us ve (Var v) t = lookupAs ve v t.
+
+    Axiom exprD_UVar : forall ve u t,
+      exprD fs us ve (UVar u) t = lookupAs us u t.
+
+    Axiom exprD_Func : forall ve f ts t,
+      exprD fs us ve (Func f ts) t =
+      match nth_error fs f with
+        | None => None
+        | Some f =>
+          match type_apply _ _ ts _ _ f.(fdenote) with
+            | None => None
+            | Some t' =>
+              @typ_cast_val _ _ (instantiate_typ ts (ftype f)) t t'
+          end
+      end.
+
+    Axiom exprD_Equal : forall ve t l r t',
+      exprD fs us ve (Equal t l r) t' =
+      match t' as t' return option (typD ts nil t') with
+        | tvProp =>
+          match exprD fs us ve l t , exprD fs us ve r t with
+            | Some l , Some r => Some (l = r)
+            | _ , _ => None
+          end
+        | _ => None
+      end.
+
+    Axiom exprD_Not : forall ve p t',
+      exprD fs us ve (Not p) t' =
+      match t' as t' return option (typD ts nil t') with
+        | tvProp =>
+          match exprD fs us ve p tvProp with
+            | Some p => Some (~p)
+            | _ => None
+          end
+        | _ => None
+      end.
+
+    Axiom exprD_Abs : forall ve t u e val,
+      exprD fs us ve (Abs t e) (tvArr t u) = Some val ->
+      forall x, exprD fs us (existT _ t x :: ve) e u = Some (val x).
+
+    Axiom exprD_App : forall ve t e arg,
+      exprD fs us ve (App e arg) t =
+      match typeof_expr (typeof_funcs fs) (typeof_env us) (typeof_env ve) e with
+        | Some (tvArr l r) =>
+          match exprD fs us ve e (tvArr l r)
+              , exprD fs us ve arg l
+              , typ_cast_typ _ (fun x => x) _ r t
+          with
+            | Some f , Some x , Some cast =>
+              Some (cast (f x))
+            | _ , _ , _ => None
+          end
+        | _ => None
+      end.
+  End with_envs.
+
+End ExprDenote.
